commit

AP/AP/HistBlind/D.lean
@@ -5,6 +5,49 @@ namespace AP
 instance : (default : DStrat).histBlind := by
   simp [DStrat.histBlind]
 
+noncomputable
+def State.dwn (s : State) : ℕ :=
+  Nat.findRaw # λ n => ∃ (d : DStrat), d.WF ∧ ∀ (a : AStrat), a.WF →
+  (sys.simulate (Strat.f ⟨a, d⟩) s n).2 ≠ 0
+
+theorem State.dwn_eq_zero_of_a_hws {s} [hs : sys.WF s] (h : s.a_hws) : s.dwn = 0 := by
+  apply Nat.findRaw_eq_zero_of
+  rw [←not_d_hws_iff, d_hws_iff_d_hws_bounded] at h
+  push_neg at h ⊢; exact h
+
+@[simp]
+theorem State.dwn_histBlind {s hist} [hs : sys.WF s] [hs' : sys.WF # s.setHist hist] :
+(s.setHist hist).dwn = s.dwn := by
+  by_cases h₁ : s.a_hws
+  · have h₂ : s.setHist hist |>.a_hws; simpa
+    rw [dwn_eq_zero_of_a_hws h₁, dwn_eq_zero_of_a_hws h₂]
+  simp at h₁
+  have H₁ : s.setHist hist |>.d_hws; simpa
+  rw [d_hws_iff_d_hws_bounded] at h₁ H₁
+  have ⟨⟨d, hd, h₂⟩, h₃⟩ := Nat.findRaw_spec' h₁
+  have ⟨⟨d', hd', H₂⟩, H₃⟩ := Nat.findRaw_spec' H₁
+  rw [←dwn] at h₂ h₃ H₂ H₃
+  generalize h₄ : s.setHist hist = s' at hs' H₂ H₃ ⊢
+  generalize hn : s.dwn = n at h₂ h₃ ⊢
+  generalize hn' : s'.dwn = n' at H₂ H₃ ⊢
+  clear h₁ H₁
+  
+  symm; by_contra H'
+  wlog H : n < n' with ih
+  · specialize @ih s' s.hist hs' d' hd' d hd s (by simp [←h₄])
+      hs _ hn' H₂ H₃ _ hn h₂ h₃ (ne_symm' H')
+    simp at H ih; exact H' # le_antisymm ih H
+  clear H'
+  
+  rename' d' => d₀
+  rename' hd' => hd₀
+  
+  suffices h : ∃ (d' : DStrat), d'.WF ∧ ∀ (a : AStrat), a.WF →
+    (sys.simulate (Strat.f ⟨a, d'⟩) s' n).2 ≠ 0
+  · specialize H₃ n h; linarith
+  
+  sorry
+
 -- #check 0 #exit
 
 theorem State.d_hws_histBlind_of_d_hws {s} [hs : sys.WF s] (h : s.d_hws) :
